

## Homework 1

### Exercise 1

a) Simplify the system (1) to one convection - diffusion equation for  $b(z, t)$ .

$$\partial_t b + \partial_z (ub) = 0, \quad u = \alpha b^2 - \beta b^3 \partial_z b \quad - (1)$$

with  $z \in [0, H]$ ,

Substituting  $u$ , we get:

$$\partial_t b + \partial_z (\alpha b^3 - \beta b^3 \partial_z b) = 0. \quad - (5)$$

$$\Rightarrow \partial_t b + 3\alpha b^2 \frac{\partial b}{\partial z} - 3\beta b^2 \left( \frac{\partial b}{\partial z} \right)^2 - \beta b^3 \frac{\partial^2 b}{\partial z^2} = 0$$

Linearize this by substituting  $b = D_0 + b'$ ,

$$\Rightarrow \frac{\partial (D_0 + b')}{\partial t} + 3\alpha (D_0 + b')^2 \frac{\partial (D_0 + b')}{\partial z} - 3\beta (D_0 + b')^2 \left( \frac{\partial (D_0 + b')}{\partial z} \right)^2 - \beta (D_0 + b')^3 \frac{\partial^2 (D_0 + b')}{\partial z^2} = 0$$

As  $D_0 = \text{constant}$ , then

$$\Rightarrow \frac{\partial b'}{\partial t} + 3\alpha (D_0 + b')^2 \frac{\partial b'}{\partial z} - 3\beta (D_0 + b')^2 \left( \frac{\partial b'}{\partial z} \right)^2 - \beta (D_0 + b')^3 \frac{\partial^2 b'}{\partial z^2} = 0$$

Considering  $b'$  is small, then the nonlinear terms involving  $b'$  can be neglected:

$$\Rightarrow \frac{\partial b'}{\partial t} + 3\alpha (D_0 + b')^2 \frac{\partial b'}{\partial z} - \beta (D_0 + b')^3 \frac{\partial^2 b'}{\partial z^2} = 0$$

$$\Rightarrow \frac{\partial b'}{\partial t} + 3\alpha (D_0^2 + 2D_0 b' + b'^2) \frac{\partial b'}{\partial z} - \beta (D_0^3 + 3D_0^2 b' + 3D_0 b'^2 + b'^3) \frac{\partial^2 b'}{\partial z^2} = 0$$

$$\Rightarrow \frac{\partial b'}{\partial t} + 3\alpha D_0^2 \frac{\partial b'}{\partial z} - \beta D_0^3 \frac{\partial^2 b'}{\partial z^2} = 0$$

— (6)

The derivative of  $b$  exists in the original equation and  $b$  is also a dependent variable of  $b$  itself, that's why they are called non-linear equation.

b)